Changed to FinRankUnif

Matroid/Extremal/Thickness.lean
@@ -3,7 +3,7 @@ import Matroid.Extremal.Covers
 set_option linter.style.longLine false
 
 variable {α : Type*} {M N M' : Matroid α} {I F X Y F' F₀ F₁ F₂ P L H H₁ H₂ H' B C D K : Set α}
-  {e f : α} {l r : ℕ} {a k : ℕ∞} {T : Set (Set α)} {ι : Type*} {i j : ι}
+  {e f : α} {l r : ℕ} {a k d : ℕ∞} {T : Set (Set α)} {ι : Type*} {i j : ι}
   {P P' : Matroid α → Set α → Prop}
 
 open Set
@@ -11,28 +11,69 @@ namespace Matroid
 
 section defs
 
---Ask about -1. Do we need M.RankPos?
+def IsThick (M : Matroid α) (d : ℕ∞) : Prop := d ≤ M.coverNumber Matroid.Nonspanning
 
-def IsThick (M : Matroid α) (d : ℕ∞) : Prop := d ≤ M.coverNumber (fun M X ↦ M.eRk X ≤ (M.eRank - 1))
+lemma IsThick_iff (M : Matroid α) (d : ℕ∞) :
+    M.IsThick d ↔ d ≤ M.coverNumber Matroid.Nonspanning := Eq.to_iff rfl
+
+lemma IsThick_iff' (M : Matroid α) (d : ℕ∞) :
+    M.IsThick d ↔ ∀ T, M.IsCover Matroid.Nonspanning T → d ≤ T.encard := by
+  sorry
+
 
 def IsThick_set (M : Matroid α) (X : Set α ) (d : ℕ∞) : Prop :=
     (M ↾ X).IsThick d
 
 lemma IsThick_set_iff (M : Matroid α) (X : Set α ) (d : ℕ∞) :
-    M.IsThick_set X d ↔ d ≤ (M ↾ X).coverNumber (fun M X ↦ M.eRk X ≤ (M.eRk X - 1)) := by
+    M.IsThick_set X d ↔ d ≤ (M ↾ X).coverNumber Matroid.Nonspanning := by
   sorry
 
-lemma IsThick_two [M.Nonempty] (M : Matroid α) : M.IsThick 2 := by
-  obtain ht | ⟨T, hT, hTe ⟩ := exists_cover M (fun M X ↦ M.eRk X ≤ (M.eRank - 1))
-  · unfold IsThick
-    rw [ ht]
-    simp
-  unfold IsThick
-  rw [←hTe]
-  have : M.IsRankCover (M.eRank - 1) T := by sorry
-  --( IsRankCover_iff_IsCover M (M.eRank - 1) T ).2 hT
-  --IsRankCover_two
-  sorry
+lemma IsThick_two (M : Matroid α) [M.Nonempty] : M.IsThick 2 := by
+  rw [M.IsThick_iff 2]
+  obtain ht | ⟨T, hT, hTe ⟩ := exists_cover M Matroid.Nonspanning
+  · rw [ ht]
+    simp only [le_top]
+  rw [← hTe ]
+  by_contra hc
+  obtain ⟨X, hX ⟩ := encard_eq_one.mp ((ENat.one_le_iff_ne_zero.mpr (encard_ne_zero.mpr
+    ( hT.nonempty ))).antisymm' (Order.le_of_lt_succ (Std.not_le.mp hc ) ) )
+  have hc1 : M.Spanning X := by
+    rw [← sUnion_singleton (s := X), ←hX, hT.sUnion_eq]
+    refine ⟨ by simp only [closure_ground], by simp only [subset_refl] ⟩
+  exact Ne.elim (fun a ↦ (hT.pProp X ( by rw [hX]; exact mem_singleton X )).not_spanning  hc1) hTe
+
+lemma IsThick.mono {d' : ℕ∞} (hTd : M.IsThick d ) (hd : d' ≤ d ) : M.IsThick d' := by sorry
+
+
+lemma IsThick_set.Minor_mon (hTXd : M.IsThick_set X d) (hNM : N ≤m M ) ( hX : X ⊆ N.E )
+    (hXne : (M ↾ X ).Nonempty) :
+    N.IsThick_set X d := by
+  rw [N.IsThick_set_iff X d]
+  obtain ⟨C, D, hC, hD, hDC, hrw ⟩ := hNM.exists_contract_indep_delete_coindep
+  have hDX : Disjoint D X := by grind
+  have hCX : Disjoint C X := by grind
+  have hg3 : (C ∩ M.closure X) ⊆ (M ↾ (X ∪ (C ∩ M.closure X))).E := by grind
+  have hne : ((M ↾ (X ∪ (C ∩ M.closure X))) ／ (C ∩ M.closure X)).Nonempty := by
+    refine (ground_nonempty_iff ((M ↾ (X ∪ C ∩ M.closure X)) ／ (C ∩ M.closure X))).mp ?_
+    simp only [contract_ground, restrict_ground_eq, union_diff_right]
+    have : (X \ C).Nonempty := by
+      rw [ Disjoint.sdiff_eq_right hCX ]
+      rwa [←(M ↾ X).ground_nonempty_iff, restrict_ground_eq] at hXne
+    refine nonempty_of_not_subset ?_
+    have : ¬X ⊆ C := by
+      exact not_subset.mpr this
+    grind
+  -- Peter?
+  have hP : (M ／ C ↾ X) = (M ／ (C ∩ M.closure X) ↾ X) := by sorry
+  have hCX' : Disjoint (C ∩ M.closure X) X := by grind
+  grw [hrw, delete_restrict_eq_restrict (M ／ C) hDX, hP,
+    M.contract_restrict_eq_restrict_contract hCX',
+    ←NonSpanningNumber_contract hg3 hne, ← NonSpanningNumber_set_closure (inter_subset_right)
+    (by grind) ]
+  exact (IsThick_set_iff M X d).mp hTXd
+
+
+
 
 
 end defs
