Matroid/Extremal/Covers.lean
@@ -598,16 +598,66 @@ lemma set_to_binom_number {a b : ℕ} (X : Set α) (hX : X.encard = b) :
     simpa
   rw [← ENat.coe_inj, ← hX, eq_comm, hXfin.encard_eq_coe_toFinset_card]
 
+-- lemma base_isCover {a : ℕ} (hr : M.eRank ≤ a + 1) (ha : 1 ≤ a) (hXfin : X.Finite)
+--     --(h : Maximal (fun Y ↦ Y ⊆ M.E ∧ (M ↾ Y).IsFiniteRankUniform (a + 1) Y.encard) X) :
+--     (h : MaximalFor (fun x ↦ x ∈ {X | X ⊆ M.E ∧ (M ↾ X).IsFiniteRankUniform (a + 1) X.encard}) encard X) :
+--     M.IsRankCover a (M.closure '' {K | K ⊆ X ∧ K.encard = a}) := by
+--   refine ⟨?_, ?_⟩
+--   · refine subset_antisymm (sUnion_subset fun K ↦ ?_) fun e he ↦ ?_
+--     · simp only [mem_image, mem_setOf_eq, forall_exists_index, and_imp]
+--       grind
+--     obtain ⟨E, hEX, hEunif⟩ := h.prop.2.exists_eq_unifOn
+--     obtain rfl : X = E := congr_arg Matroid.E hEunif
+--     by_contra! hcon
+--     simp only [sUnion_image, mem_setOf_eq, mem_iUnion, exists_prop, not_exists, not_and,
+--       and_imp] at hcon
+--     have hcon' (Z) (hZ : Z ⊆ X) (hZa : Z.encard ≤ a) : e ∉ M.closure Z := by
+--       have haX : a ≤ X.encard := by
+--         grw [← M.restrict_ground_eq (R := X), ← eRank_le_encard_ground, h.prop.2.eRank_eq]
+--         simp
+--       obtain ⟨W, hZW, hWZ, hW⟩ := exists_superset_subset_encard_eq hZ hZa haX
+--       exact notMem_subset (M.closure_subset_closure hZW) (hcon W hWZ hW)
+--     have heX : e ∉ X := by
+--       by_contra hc
+--       exact hcon' (singleton e) (singleton_subset_iff.mpr hc )
+--         (by simp only [encard_singleton, ENat.one_le_coe, ha ]) (mem_closure_self M e he )
+--     --have hwin := h.not_prop_of_ssuperset (t := insert e X) (by grind)
+--     have hwin := h.not_prop_of_gt (j := insert e X)
+--       (Finite.encard_lt_encard hXfin (ssubset_insert heX ))
+--     simp only [mem_setOf_eq, not_and, insert_subset_iff.mpr ⟨he, h.prop.1 ⟩,forall_const ] at hwin
+--     --rw [insert_subset_iff , and_iff_right he, and_iff_right h.prop.1] at hwin
+--     apply hwin
+--     suffices aux : (M ↾ insert e X) = unifOn (insert e X) (a + 1) by
+--       rw [aux]
+--       apply unifOn_isFiniteRank_uniform
+--       grw [h.prop.2.le, ← subset_insert]
+--     refine ext_indep rfl fun I (hI : I ⊆ insert e X) ↦ ?_
+--     simp only [restrict_indep_iff, hI, and_true, unifOn_indep_iff, Nat.cast_add, Nat.cast_one]
+--     refine ⟨fun hIi ↦ by grw [hIi.encard_le_eRank, hr], fun hcard ↦ ?_⟩
+--     have hI₀ : M.Indep (I \ {e}) := by
+--       have hrestr := (M.restrict_indep_iff (R := X) (I := I \ {e})).1
+--       nth_grw 1 [hEunif, unifOn_indep_iff, diff_subset] at hrestr
+--       grind
+--     by_cases! heI : e ∉ I
+--     · rwa [diff_singleton_eq_self heI] at hI₀
+--     rw [← insert_diff_self_of_mem heI, hI₀.insert_indep_iff_of_notMem (by grind), mem_diff,
+--       and_iff_right he]
+--     refine hcon'  _ (by grind) ?_
+--     grw [← ENat.add_one_le_add_one_iff, ← hcard, encard_diff_singleton_add_one heI]
+--   simp only [mem_image, mem_setOf_eq, forall_exists_index, and_imp]
+--   rintro F I hI hcard rfl
+--   grw [eRk_closure_eq, eRk_le_encard, hcard]
+
 lemma base_isCover {a : ℕ} (hr : M.eRank ≤ a + 1) (ha : 1 ≤ a) (hXfin : X.Finite)
     --(h : Maximal (fun Y ↦ Y ⊆ M.E ∧ (M ↾ Y).IsFiniteRankUniform (a + 1) Y.encard) X) :
-    (h : MaximalFor (fun x ↦ x ∈ {X | X ⊆ M.E ∧ (M ↾ X).IsFiniteRankUniform (a + 1) X.encard}) encard X) :
+    (h : MaximalFor (fun x ↦ x ∈ {X | X ⊆ M.E ∧ (M ↾ X).IsFinRankUniform (a + 1) }) encard X) :
     M.IsRankCover a (M.closure '' {K | K ⊆ X ∧ K.encard = a}) := by
   refine ⟨?_, ?_⟩
   · refine subset_antisymm (sUnion_subset fun K ↦ ?_) fun e he ↦ ?_
     · simp only [mem_image, mem_setOf_eq, forall_exists_index, and_imp]
       grind
     obtain ⟨E, hEX, hEunif⟩ := h.prop.2.exists_eq_unifOn
-    obtain rfl : X = E := congr_arg Matroid.E hEunif
+    --obtain rfl : X = E := congr_arg Matroid.E hEunif
     by_contra! hcon
     simp only [sUnion_image, mem_setOf_eq, mem_iUnion, exists_prop, not_exists, not_and,
       and_imp] at hcon
@@ -629,14 +679,18 @@ lemma base_isCover {a : ℕ} (hr : M.eRank ≤ a + 1) (ha : 1 ≤ a) (hXfin : X.
     apply hwin
     suffices aux : (M ↾ insert e X) = unifOn (insert e X) (a + 1) by
       rw [aux]
-      apply unifOn_isFiniteRank_uniform
-      grw [h.prop.2.le, ← subset_insert]
+      apply unifOn_isFinRankUniform
+      grw [h.prop.2.le , ← subset_insert]
+      exact encard_le_encard fun ⦃a⦄ a_1 ↦ a_1
     refine ext_indep rfl fun I (hI : I ⊆ insert e X) ↦ ?_
     simp only [restrict_indep_iff, hI, and_true, unifOn_indep_iff, Nat.cast_add, Nat.cast_one]
     refine ⟨fun hIi ↦ by grw [hIi.encard_le_eRank, hr], fun hcard ↦ ?_⟩
     have hI₀ : M.Indep (I \ {e}) := by
       have hrestr := (M.restrict_indep_iff (R := X) (I := I \ {e})).1
-      nth_grw 1 [hEunif, unifOn_indep_iff, diff_subset] at hrestr
+      have : I \ {e} ⊆ E  := by
+        rw [ ←unifOn_ground_eq E (k := a + 1), ← hEX, restrict_ground_eq, diff_subset_iff, singleton_union]
+        exact LE.le.subset hI
+      nth_grw 1 [hEX, unifOn_indep_iff, diff_subset] at hrestr
       grind
     by_cases! heI : e ∉ I
     · rwa [diff_singleton_eq_self heI] at hI₀
@@ -655,9 +709,9 @@ lemma baseCase {a b : ℕ} (ha : 1 ≤ a) (hM : NoUniformMinor M (a + 1) (b + 1)
       (Exists.intro ((fun x1 x2 ↦ x1 + x2) a 1) (hr.symm)))
   by_contra! hcon
   obtain ⟨B, hB⟩ := M.exists_isBase
-  set Unif : Set (Set α) := {X | X ⊆ M.E ∧ (M ↾ X).IsFiniteRankUniform (a + 1) X.encard} with h_UnifS
+  set Unif : Set (Set α) := {X | X ⊆ M.E ∧ (M ↾ X).IsFinRankUniform (a + 1) } with h_UnifS
   have hne : Unif.Nonempty := by
-    refine ⟨B, (IsBase.subset_ground hB), rfl, ?_, ?_⟩
+    refine ⟨B, (IsBase.subset_ground hB), ?_, ?_,⟩
     · rwa [eRank_restrict, hB.eRk_eq_eRank]
     rw [hB.indep.restrict_eq_freeOn]
     exact freeOn_uniform B
@@ -665,9 +719,16 @@ lemma baseCase {a b : ℕ} (ha : 1 ≤ a) (hM : NoUniformMinor M (a + 1) (b + 1)
     intro X hX
     by_contra hc
     simp only [not_lt] at hc
+    --have : X ⊆ M.E := by exact hX.1
+    have h2 : ((unifOn (M ↾ X).E (a + 1)).NoUniformMinor (a + 1) (b + 1)) := by
+      rw[←hX.2.eq_unifOn ]
+      exact hM.minor (IsRestriction.isMinor (restrict_isRestriction M X) )
+    have h3 := unifOn_noUniformMinor_iff.1 h2
+    grw [← restrict_ground_eq (M := M) (R := X)] at hc
+    grind
     --simp only [mem_setOf_eq] at hX
-    exact hc.not_gt <| hM.lt_of_isoMinor (N := M ↾ X) (b' := X.encard)
-      (restrict_isRestriction _ _ hX.1).isMinor.isoMinor hX.2
+    -- exact hc.not_gt <| hM.lt_of_isoMinor (N := M ↾ X) (b' := X.encard)
+    --   (restrict_isRestriction _ _ hX.1).isMinor.isoMinor sorry
   have hcard : (encard '' Unif).Finite := by
     refine ENat.finite_of_sSup_lt_top ?_
     refine lt_of_le_of_lt ?_ <| WithTop.natCast_lt_top (b + 1)
@@ -688,7 +749,7 @@ lemma baseCase {a b : ℕ} (ha : 1 ≤ a) (hM : NoUniformMinor M (a + 1) (b + 1)
     (Nat.choose_le_choose a (Nat.le_of_lt_succ (ENat.coe_lt_coe.mp hXb )))] at hcon
   simp only [lt_self_iff_false] at hcon
 
-lemma coverNumber_rank_Frombase [M.RankFinite] {a b : ℕ} (ha : 1 ≤ a)
+lemma coverNumber_rank_Frombase {a b : ℕ} (ha : 1 ≤ a)
     (hM : NoUniformMinor M ( a + 1 ) (b + 1)) :
     M.coverNumber (fun M X ↦ M.eRk X ≤ a) ≤
     (Nat.choose b a) * M.coverNumber (fun M X ↦ M.eRk X ≤ (a + 1)) := by
@@ -764,25 +825,233 @@ lemma coverNumber_Bound_contract [M.RankFinite] {a b : ℕ} (ha : 1 ≤ a)
 
 
 -- change `ha` to `a ≠ 0`.
-lemma coverNumber_Bound_contract' {M : Matroid α} {C : Set α} {a b : ℕ} (ha : 1 ≤ a)
+lemma coverNumber_Bound_contract' {M : Matroid α} {C : Set α} {a b : ℕ} (ha : a ≠ 0) (hb : a ≤ b)
     (hM : NoUniformMinor M (a + 1) (b + 1)) (hC : C ⊂ M.E)  :
     M.coverNumber (fun M X ↦ M.eRk X ≤ a) ≤
     (Nat.choose b a)^(M.eRk C) * (M ／ C).coverNumber (fun M X ↦ M.eRk X ≤ a) := by
   obtain htop | hlt := eq_or_ne (M.eRk C) ⊤
-  · sorry
+  · grw [htop, ENat.epow_top, ENat.top_mul, ← le_top ]
+    · have heN : (M／ C).Nonempty := by
+        rw[←(M／ C).ground_nonempty_iff, contract_ground]
+        exact (Set.nonempty_of_ssubset (by grind ) )
+      exact ENat.one_le_iff_ne_zero.mp (coverNumer_positive (fun M X ↦ M.eRk X ≤ a) )
+    obtain rfl | hlt := hb.eq_or_lt
+    · simp [noUniformMinor_self_iff] at hM
+      grw [ ←eRk_le_eRank M C, htop ] at hM
+      simp only [not_top_lt] at hM
+    rw [← ENat.coe_one, ENat.coe_lt_coe]
+    suffices b.choose a ≠ 0 ∧ b.choose a ≠ 1 by lia
+    exact ⟨(Nat.choose_pos hlt.le).ne.symm, by simp [Nat.choose_eq_one_iff, hlt.ne.symm, ha] ⟩
   have hresP : (M ↾ C).RankPos := sorry
     -- (eRank_ne_zero_iff (M ↾ C)).mp <| by simp [eRank_restrict, ne_eq, ← hn]
   obtain ⟨e, heC⟩ : ∃ e, (M ↾ C).IsNonloop e := exists_isNonloop (M ↾ C)
   rw [restrict_isNonloop_iff] at heC
-  have h' : (M ／ {e}).eRk (C \ {e}) < M.eRk C := sorry
-  have ih := coverNumber_Bound_contract' (M := M ／ {e}) (C := C \ {e}) (a := a) (b := b) ha sorry
-    sorry
-  sorry
+  -- have hrelrk := IsNonloop.eRelRk_add_one_eq heC.1 (C \ {e})
+  -- simp only [insert_diff_singleton, insert_eq_of_mem heC.2] at hrelrk
+  have h' : (M ／ {e}).eRk (C \ {e}) < M.eRk C := by
+    have hrelrk := IsNonloop.eRelRk_add_one_eq heC.1 (C \ {e})
+    simp only [insert_diff_singleton, insert_eq_of_mem heC.2] at hrelrk
+    rw [ ←hrelrk, eRelRk.eq_1 ]
+    simp only [ENat.lt_add_left_iff, ne_eq, eRk_eq_top_iff, IsRkFinite.diff_singleton_iff, not_not,
+      one_ne_zero, not_false_eq_true, and_true]
+    rw [ IsRkFinite ]
+    refine eRank_lt_top_iff.mp ?_
+    grw [eRank_restrict, eRk_contract_le_eRk M {e} C]
+    exact Ne.lt_top' (id (Ne.symm hlt))
+  have hsub1 : (C \ {e}) ⊂ (M／ {e}).E := by
+    simp only [contract_ground]
+    refine Set.ssubset_iff_subset_ne.mpr ⟨diff_subset_diff_left (subset_of_ssubset hC), ?_ ⟩
+    by_contra hc
+    have h : C = M.E := by
+      rw [←insert_diff_self_of_mem heC.2, ←insert_diff_self_of_mem heC.1.mem_ground, hc]
+    grind
+  have heN : (M／ {e}).Nonempty := by
+    rw[←(M／ {e}).ground_nonempty_iff, contract_ground]
+    exact (Set.nonempty_of_ssubset (by grind ) )
+  have : 1 ≤ a := by exact Nat.one_le_iff_ne_zero.mpr ha
+  have ih := coverNumber_Bound_contract' (M := M ／ {e}) (C := C \ {e}) (a := a) (b := b) ha
+    hb (hM.minor (contract_isMinor M {e} )) hsub1
+  grw [coverNumber_rank_Frombase (Nat.one_le_iff_ne_zero.mpr ha) hM, coverNumber_contract_one (heC.1.mem_ground ) heC.1 heN, ih ]
+  simp only [contract_contract, union_diff_self, singleton_union, ge_iff_le, insert_eq_of_mem heC.2,
+    ←mul_assoc]
+  nth_rw 1 [←eRelRk.eq_1, ←ENat.epow_one (x := ↑(b.choose a)),
+    ←ENat.epow_add (x :=  ↑(b.choose a)) (y := 1) (z := (M.eRelRk {e} (C \ {e})) ),
+    ←add_comm (a := (M.eRelRk {e} (C \ {e}))) (b:= 1 ), (heC.1).eRelRk_add_one_eq, insert_diff_singleton, insert_eq_of_mem heC.2 ]
 termination_by M.eRk C
 
 
 end Rank
 
+section NonSpanning
+
+lemma NonSpanning_to_RankCover [M.RankFinite] (hM : 2 ≤ M.eRank) :
+    M.IsCover Matroid.Nonspanning T ↔ M.IsRankCover (M.eRank - 1) T := by
+  refine ⟨?_, ?_ ⟩
+  · intro h
+    refine ⟨ h.sUnion_eq, ?_ ⟩
+    intro F hF
+    by_contra hc
+    simp only [not_le] at hc
+    have : M.eRank ≤ M.eRk F := by
+      have : M.eRank - 1 + 1 ≤  M.eRk F := by exact Order.add_one_le_of_lt hc
+      sorry
+    sorry
+  sorry
+
+lemma NonSpaning_le_two [M.Nonempty] (hle : M.eRank ≤ 1) :
+    ⊤ ≤ M.coverNumber (Matroid.Nonspanning) := by
+  obtain hT | ⟨T, hT1, hT2 ⟩  := M.exists_cover (Matroid.Nonspanning)
+  · rw[ hT ]
+  by_contra hc
+  have : M.RankFinite := by
+    refine eRank_lt_top_iff.mp ?_
+    grw[hle]
+    exact ENat.one_lt_top
+  have hu := hT1.sUnion_eq
+  have hl : ∀ T1 ∈ T, T1 ⊆ M.loops := by
+    intro T1 hT'
+    have h1 : M.eRk T1 < M.eRank := Nonspanning.eRk_lt (hT1.pProp T1 hT' )
+    grw [hle] at h1
+    simp only [ENat.lt_one_iff] at h1
+    exact (M.eRk_eq_zero_iff (X := T1) (hX := by grind)).1 h1
+  have hs : M.E ⊆ M.loops := by
+    rw [←hT1.sUnion_eq]
+    exact sUnion_subset hl
+  obtain ⟨T', hT' ⟩ := hT1.nonempty
+  have h2 : M.E ⊆ M.closure T' := by
+    grw [hs]
+    exact loops_subset_closure M T'
+  exact Ne.elim (fun a ↦ ((hT1.pProp T' hT').not_spanning) ((spanning_iff_ground_subset_closure
+    (hT1.subset_ground hT') ).2 h2)) hT2
+
+
+lemma Non_spanning_singleton (he : e ∈ M.E) (hM : 2 ≤ M.eRank) : M.Nonspanning {e} := by
+    by_contra hc
+    have h1 : M.eRank ≤ 1 := by
+      rw [not_nonspanning_iff] at hc
+      rw [←hc.eRk_eq]
+      simp only [eRk_singleton_le]
+    grw [←hM] at h1
+    simp only [ENat.not_ofNat_le_one] at h1
+
+lemma IsCover_singleton_NonSpanning (hM : 2 ≤ M.eRank) :
+    M.IsCover (Matroid.Nonspanning) (singleton '' M.E) := by
+  exact IsCover_singleton_Prop (fun e he ↦ Non_spanning_singleton he hM)
+
+lemma IsCover_singleton_le_NonSpanning (hM : 2 ≤ M.eRank) :
+    M.coverNumber (Matroid.Nonspanning) ≤ M.E.encard := by
+  exact IsCover_singleton_le (fun e he ↦ Non_spanning_singleton he hM)
+
+lemma NonSpaning_cover_exists (hM : 2 ≤ M.eRank) : M.hasCover_with Matroid.Nonspanning := by
+  refine ⟨(singleton '' M.E), IsCover_singleton_NonSpanning hM ⟩
+
+lemma IsNonSpaningCover_contract (h : (M ／ X).IsCover (Matroid.Nonspanning) T)
+    (hX : X ⊆ M.E) (hXN : (M ／ X).Nonempty) :
+    M.IsCover (Matroid.Nonspanning) ((· ∪ X) '' T) := by
+  apply h.contract hX hXN
+  intro Y hC
+  refine ⟨ ?_, union_subset (by have := hC.subset_ground; grind ) hX  ⟩
+  · by_contra hc
+    have hcc : (M ／ X).Spanning Y := by
+      have h1 := hc.contract X
+      simp only [union_diff_right] at h1
+      exact h1.superset (diff_subset (s := Y) (t := X)) (hC.subset_ground)
+    rw [←not_spanning_iff hcc.subset_ground ] at hC
+    exact (iff_false_intro hC).mp hcc
+
+lemma NonSpanningNumber_contract (hX : X ⊆ M.E) (hne : (M ／ X).Nonempty) :
+    M.coverNumber Matroid.Nonspanning ≤ (M ／ X).coverNumber Matroid.Nonspanning := by
+  obtain hT | ⟨T, hT, hTe ⟩ := (M ／ X).exists_cover (Matroid.Nonspanning)
+  · rw [hT]
+    exact OrderTop.le_top (M.coverNumber Nonspanning)
+  rw [← hTe]
+  exact
+    Std.IsPreorder.le_trans (M.coverNumber Nonspanning) ((fun x ↦ x ∪ X) '' T).encard T.encard
+      ((IsNonSpaningCover_contract hT hX hne).coverNumber_le)
+      (encard_image_le (fun x ↦ x ∪ X) T )
+
+lemma NonSpanningNumber_set_closure (hY : Y ⊆ M.closure X) (hX : X ⊆ M.E) :
+    (M ↾ X).coverNumber Nonspanning  ≤ (M ↾ (X ∪ Y)).coverNumber Nonspanning := by
+  obtain hT | ⟨T, hT, hTe ⟩ := (M ↾ (X ∪ Y)).exists_cover (Matroid.Nonspanning)
+  · rw [hT]
+    exact OrderTop.le_top ((M ↾ X).coverNumber Nonspanning)
+  rw[←hTe]
+  have hcov : (M ↾ X).IsCover (Matroid.Nonspanning) ((fun x ↦ x ∩ X) '' T) := by
+    refine ⟨?_, ?_ ⟩
+    · refine subset_antisymm (sUnion_subset fun K ↦ ?_) fun e he ↦ ?_
+      · intro hK
+        obtain ⟨K', hK'T, hK' ⟩ := hK
+        rw [← hK']
+        grind
+      have h1 := hT.sUnion_eq
+      simp only [restrict_ground_eq] at h1
+      simp only [restrict_ground_eq] at he
+      have : e ∈  ⋃₀ T := by grind
+      obtain ⟨ T', hT', heT' ⟩ := this
+      have : e ∈ T' ∩ X := by grind
+      grind
+    intro F hF
+    obtain ⟨F', hF', hhF' ⟩ := hF
+    simp only at hhF'
+    rw [← hhF']
+    by_contra hc
+    rw [not_nonspanning_iff, restrict_spanning_iff (by grind)] at hc
+    have hcc : X ∪ Y ⊆ M.closure F' := union_subset (LE.le.subset fun ⦃a⦄ a_1 ↦
+      (closure_subset_closure M (inter_subset_left )) (hc a_1)) ( LE.le.subset fun ⦃a⦄ a_1 ↦
+      (closure_subset_closure M (inter_subset_left )) ((LE.le.subset fun ⦃a⦄ a_1 ↦
+      (closure_subset_closure_of_subset_closure hc ) (hY a_1) ) a_1))
+    rw [←restrict_spanning_iff (hR := by grind), ←not_nonspanning_iff (by grind)  ] at hcc
+    exact Ne.elim (fun a ↦ hcc (hT.pProp F' hF')) hTe
+    exact LE.le.subset (hT.subset_ground hF')
+  grw [hcov.coverNumber_le ]
+  exact encard_image_le (fun x ↦ x ∩ X) T
+
+
+
+-- lemma NonSpaningNumber_delete_loop (hne : (M ＼ D).Nonempty) (hk : 1 ≤ k) (hD : D ⊆ M.loops ) :
+--     M.coverNumber (fun M X ↦ M.eRk X ≤ k) = (M ＼ D).coverNumber (fun M X ↦ M.eRk X ≤ k) := by
+
+--   sorry
+  -- obtain ⟨T, hT, hTen ⟩ := exists_min_cover (RankPropCover_exists (M := M) hk )
+  -- have h1 := (hT.delete D ).coverNumber_le
+  -- grw[encard_image_le (fun s ↦ s \ D) T, hTen ] at h1
+  -- obtain ⟨T', hT', hT'en ⟩ := exists_min_cover (RankPropCover_exists (M := (M ＼ D)) hk )
+  -- have hcov : M.IsCover (fun M X ↦ M.eRk X ≤ k) (M.closure '' T' ) := by
+  --   refine ⟨ ?_, ?_ ⟩
+  --   · refine subset_antisymm (sUnion_subset fun K ↦ ?_) fun e he ↦ ?_
+  --     · simp only [mem_image, forall_exists_index, and_imp]
+  --       grind
+  --     by_cases heD : e ∈ D
+  --     · obtain ⟨ X, hX ⟩ := hT'.nonempty
+  --       have := (IsLoop.mem_closure (hD heD) X )
+  --       grind
+  --     have h2 : e ∈ M.E \ D := mem_diff_of_mem he heD
+  --     rw[←delete_ground,  ←hT'.sUnion_eq  ] at h2
+  --     obtain ⟨ X, hX, heX ⟩ := h2
+  --     have := (mem_closure_of_mem' M heX he )
+  --     grind
+  --   intro F hF
+  --   obtain ⟨F' ,hF', hF2 ⟩ := hF
+  --   rw[←hF2, eRk_closure_eq M F']
+  --   have ha := hT'.pProp F' hF'
+  --   simp only [delete_eRk_eq'] at ha
+  --   have ha1 : F' \ D = F' := by
+  --     have := hT'.subset_ground hF'
+  --     grind
+  --   rwa [ha1] at ha
+  -- have h2 := hcov.coverNumber_le
+  -- grw [encard_image_le M.closure T', hT'en] at h2
+  -- grind
+
+-- lemma NonSpaningNumber_contract_loop (hne : (M ＼ D).Nonempty) (hk : 1 ≤ k) (hD : D ⊆ M.loops ) :
+--     M.coverNumber (fun M X ↦ M.eRk X ≤ k) = (M ／ D).coverNumber (fun M X ↦ M.eRk X ≤ k) := by
+--   rw[contract_eq_delete_of_subset_loops hD]
+--   exact coverNumber_delete_loop hne hk hD
+
+
+
+
+end NonSpanning
 
 
 
@@ -795,45 +1064,44 @@ end Rank
 
 
 
+-- section Indexed
 
-section Indexed
+-- variable {T : ι → Set α}
 
-variable {T : ι → Set α}
+-- @[mk_iff]
+-- structure IsIndexedCover (M : Matroid α) (k : ℕ∞) (T : ι → Set α) : Prop where
+--   iUnion_eq : ⋃ i, T i = M.E
+--   eRk_le : ∀ i, M.eRk (T i) ≤ k
 
-@[mk_iff]
-structure IsIndexedCover (M : Matroid α) (k : ℕ∞) (T : ι → Set α) : Prop where
-  iUnion_eq : ⋃ i, T i = M.E
-  eRk_le : ∀ i, M.eRk (T i) ≤ k
+-- lemma IsIndexedCover.subset_ground (h : M.IsIndexedCover k T) (i : ι) : T i ⊆ M.E := by
+--   grw [← h.iUnion_eq, ← subset_iUnion]
 
-lemma IsIndexedCover.subset_ground (h : M.IsIndexedCover k T) (i : ι) : T i ⊆ M.E := by
-  grw [← h.iUnion_eq, ← subset_iUnion]
+-- lemma IsIndexedCover.isIndexedCover_closure (h : M.IsIndexedCover k T) :
+--     M.IsIndexedCover k (fun i ↦ M.closure (T i)) := by
+--   refine ⟨(iUnion_subset (fun i ↦ M.closure_subset_ground ..)).antisymm ?_, fun i ↦ ?_⟩
+--   · grw [← h.iUnion_eq, iUnion_mono (fun i ↦ M.subset_closure (T i) (h.subset_ground i))]
+--   simpa using h.eRk_le i
 
-lemma IsIndexedCover.isIndexedCover_closure (h : M.IsIndexedCover k T) :
-    M.IsIndexedCover k (fun i ↦ M.closure (T i)) := by
-  refine ⟨(iUnion_subset (fun i ↦ M.closure_subset_ground ..)).antisymm ?_, fun i ↦ ?_⟩
-  · grw [← h.iUnion_eq, iUnion_mono (fun i ↦ M.subset_closure (T i) (h.subset_ground i))]
-  simpa using h.eRk_le i
+-- lemma setOf_point_isIndexedCover (M : Matroid α) [M.RankPos] :
+--     M.IsIndexedCover 1 (fun x : {P // M.IsPoint P} ↦ x.1) := by
+--   refine ⟨(iUnion_subset fun P ↦ P.2.subset_ground).antisymm fun e he ↦ ?_, ?_⟩
+--   · obtain hl | hnl := M.isLoop_or_isNonloop e
+--     · obtain ⟨f, hf⟩ := M.exists_isNonloop
+--       exact mem_iUnion_of_mem (i := ⟨M.closure {f}, hf.closure_isPoint⟩) <| hl.mem_closure {f}
+--     exact mem_iUnion_of_mem (i := ⟨M.closure {e}, hnl.closure_isPoint⟩) <| M.mem_closure_self e
+--   simp +contextual [IsPoint.eRk]
 
-lemma setOf_point_isIndexedCover (M : Matroid α) [M.RankPos] :
-    M.IsIndexedCover 1 (fun x : {P // M.IsPoint P} ↦ x.1) := by
-  refine ⟨(iUnion_subset fun P ↦ P.2.subset_ground).antisymm fun e he ↦ ?_, ?_⟩
-  · obtain hl | hnl := M.isLoop_or_isNonloop e
-    · obtain ⟨f, hf⟩ := M.exists_isNonloop
-      exact mem_iUnion_of_mem (i := ⟨M.closure {f}, hf.closure_isPoint⟩) <| hl.mem_closure {f}
-    exact mem_iUnion_of_mem (i := ⟨M.closure {e}, hnl.closure_isPoint⟩) <| M.mem_closure_self e
-  simp +contextual [IsPoint.eRk]
-
-lemma IsIndexedCover.cover_cover {η : ι → Type*} (h : M.IsIndexedCover k T)
-    (T₀ : (i : ι) → (η i) → Set α) (hT₀ : ∀ i, (M ↾ (T i)).IsIndexedCover a (T₀ i)) :
-    M.IsIndexedCover a (fun i : ((i : ι) × η i) ↦ T₀ i.1 i.2) := by
-  refine ⟨?_, ?_⟩
-  · rw [← h.iUnion_eq, iUnion_sigma]
-    refine iUnion_congr fun i ↦ ?_
-    rw [(hT₀ i).iUnion_eq, restrict_ground_eq]
-  rintro ⟨i, j⟩
-  have := (hT₀ i).eRk_le j
-  rwa [restrict_eRk_eq', inter_eq_self_of_subset_left] at this
-  grw [(hT₀ i).subset_ground, restrict_ground_eq]
+-- lemma IsIndexedCover.cover_cover {η : ι → Type*} (h : M.IsIndexedCover k T)
+--     (T₀ : (i : ι) → (η i) → Set α) (hT₀ : ∀ i, (M ↾ (T i)).IsIndexedCover a (T₀ i)) :
+--     M.IsIndexedCover a (fun i : ((i : ι) × η i) ↦ T₀ i.1 i.2) := by
+--   refine ⟨?_, ?_⟩
+--   · rw [← h.iUnion_eq, iUnion_sigma]
+--     refine iUnion_congr fun i ↦ ?_
+--     rw [(hT₀ i).iUnion_eq, restrict_ground_eq]
+--   rintro ⟨i, j⟩
+--   have := (hT₀ i).eRk_le j
+--   rwa [restrict_eRk_eq', inter_eq_self_of_subset_left] at this
+--   grw [(hT₀ i).subset_ground, restrict_ground_eq]
 
 
 
